\section{Aufgabe 3}
    \subsection{a)}
        $$f(x) = 0 \Leftrightarrow x^6-x^2 = 0$$
        $$\Leftrightarrow x^2(x^4-1) = 0$$
        $$\Leftrightarrow x^2(x^2-1)(x^2+1) = 0$$
        $$\Leftrightarrow x^2(x^2+1)(x+1)(x-1) = 0$$
        $\Rightarrow x_1 = 0, x_2 = -1, x_3 = 1, x_4 = i, x_5 = -i$

    \subsection{b)}
        $$f(x) = 0 \Leftrightarrow x^3+4x^2-7x+2 = 0$$
        Durch geschicktes Hinsehen bekommen wir $x_1 = 1$, wodurch wir im folgenden Schritt den Term aufteilen k√∂nnen in:
        $$\Rightarrow (x-1)(x^2+5x-2) = 0$$
        $$\Rightarrow (x-1) = 0 \lor x^2+5x-2 = 0$$
        $$\Rightarrow x_{2,3} = \frac{-5 \pm \sqrt{5^2-4\cdot 1 \cdot (-2)}}{2}$$
        $$\Leftrightarrow x_{2,3} = \frac{-5 \pm \sqrt{33}}{2}$$
        $$\Rightarrow x_2 = \frac{-5 + \sqrt{33}}{2} \land x_3 = \frac{-5 - \sqrt{33}}{2}$$
        