\section{Aufgabe 4}
Wir wissen bereits: $cosh(x) = \frac{e^x+e^{-x}}{2}$ und wir wissen auch $ e^x = \sum_{n=0}^{\infty}\frac{x^n}{n!}$. \\
Wir wollen nun diese beiden Gleichungs so kombinieren, dass wir $cosh(x) = \sum_{i=0}^{\infty} \frac{x^{2n}}{2n!} $ bekommen
$$\Rightarrow 
cosh(x) = \frac{e^x+e^{-x}}{2} 
= \frac{\sum_{n=0}^{\infty}\frac{x^n}{n!} + \sum_{n=0}^{\infty}\frac{-x^n}{n!}}{2} 
$$
$$
= \frac{\sum_{n=0}^{\infty}\frac{x^2n}{2n!} + \sum_{n=0}^{\infty}\frac{x^2n+1}{(2n+1)!} + \sum_{n=0}^{\infty}\frac{x^2n}{2n!} - \sum_{n=0}^{\infty}\frac{x^2n+1}{(2n+1)!}}{2}
$$
$$= \frac{2 \cdot \sum_{n=0}^{\infty}\frac{x^2n}{2n!} }{2} = \sum_{n=0}^{\infty}\frac{x^2n}{2n!}$$
$$\Rightarrow cosh(x) = \sum_{n=0}^{\infty}\frac{x^2n}{2n!}$$